src/Assembly/Pipeline.v
@@ -1,79 +1,61 @@
-Require Import Bedrock.Word.
-Require Import Crypto.Assembly.QhasmCommon Crypto.Assembly.QhasmEvalCommon.
-Require Import Crypto.Assembly.Pseudo Crypto.Assembly.Qhasm Crypto.Assembly.AlmostQhasm Crypto.Assembly.Conversion Crypto.Assembly.Language.
-Require Import Crypto.Assembly.PseudoConversion Crypto.Assembly.AlmostConversion Crypto.Assembly.StringConversion.
-Require Import Crypto.Assembly.Pseudize.
+Require Import Crypto.Assembly.PhoasCommon.
+Require Import Crypto.Assembly.HL.
+Require Import Crypto.Assembly.LL.
+Require Import Crypto.Assembly.Compile.
+Require Import Crypto.Assembly.Conversions.
+Require Import Crypto.Assembly.StringConversion.
+Require Import Crypto.Assembly.State.
 Require Import Crypto.Util.Notations.
 
-Module Pipeline.
-  Export AlmostQhasm Qhasm QhasmString.
-  Export Pseudo.
+Module GF25519.
+  Import ListNotations StateCommon EvalUtil ListState.
+  Import HL LL.
 
-  Transparent Pseudo.Program AlmostQhasm.Program Qhasm.Program QhasmString.Program.
-  Transparent Pseudo.Params AlmostQhasm.Params Qhasm.Params QhasmString.Params.
+  Local Infix ">>" := Z.shiftr.
+  Local Infix "&" := (fun x y => Z.land x (Z.of_nat (Z.to_nat y))).
+  Local Open Scope Z_scope.
+  Require Import Crypto.Spec.ModularArithmetic.
+  Require Import Crypto.CompleteEdwardsCurve.ExtendedCoordinates.
+  Require Import Crypto.Specific.GF25519.
+  Require Import Crypto.Experiments.SpecEd25519.
 
-  Definition toAlmost {w s n m} (p: @Pseudo w s n m) : option AlmostProgram :=
-    PseudoConversion.convertProgram (mkParams w s n m) tt p.
+  (* Computing the length first is necessary to make this run in tolerable time on 8.6 *)
+  Definition twice_d' := Eval cbv [length params25519 ModularBaseSystemOpt.limb_widths_from_len ModularBaseSystem.encode ModularBaseSystemList.encode PseudoMersenneBaseParams.limb_widths] in ModularBaseSystem.encode(modulus:=q) (d + d)%F.
+  Definition twice_d : fe25519 := Eval vm_compute in twice_d'.
 
-  Definition toQhasm {w s n m} (p: @Pseudo w s n m) : option (list QhasmStatement) :=
-    omap (toAlmost p) (AlmostConversion.convertProgram tt tt).
+  Definition ge25519_add' :=
+    Eval cbv beta delta [Extended.add_coordinates fe25519 add mul sub ModularBaseSystemOpt.Let_In twice_d] in
+      @Extended.add_coordinates fe25519 add sub mul twice_d.
 
-  Definition toString {w s n m} (p: @Pseudo w s n m) : option string :=
-    omap (toQhasm p) (StringConversion.convertProgram tt tt).
-End Pipeline.
-
-Module PipelineExamples.
-  Import Pipeline ListNotations StateCommon EvalUtil ListState.
-
-  Local Notation "v [[ i ]]" := (nth i v (wzero _)).
-  Local Notation "$$ v" := (natToWord _ v).
-
-  (*
-  Definition add_example: @pseudeq 32 W32 1 1 (fun v =>
-      plet a := $$ 1 in
-      plet b := v[[0]] in
-      [a ^+ b]).
-    pseudo_solve.
+  Definition ResultType: type.
+  Proof.
+    let T' := type of (twice_d, twice_d, twice_d, twice_d) in
+    let T := eval vm_compute in T' in
+    let t := reify_type T in
+    exact t.
   Defined.
 
-  Definition add_ex_str :=
-    (Pipeline.toString (proj1_sig add_example)).
+  (* Too slow for CI
 
-  Definition and_example: @pseudeq 32 W32 1 1 (fun v =>
-      plet a := $$ 1 in
-      plet b := v[[0]] in
-      [a ^& b]).
-    pseudo_solve.
+  Definition ge25519_ast P Q : { r: @Expr Z ResultType | ZInterp r = ge25519_add' P Q }.
+  Proof.
+    refine (
+let '((P_X_0, P_X_1, P_X_2, P_X_3, P_X_4, P_X_5, P_X_6, P_X_7, P_X_8, P_X_9), (P_Y_0, P_Y_1, P_Y_2, P_Y_3, P_Y_4, P_Y_5, P_Y_6, P_Y_7, P_Y_8, P_Y_9), (P_Z_0, P_Z_1, P_Z_2, P_Z_3, P_Z_4, P_Z_5, P_Z_6, P_Z_7, P_Z_8, P_Z_9), (P_T_0, P_T_1, P_T_2, P_T_3, P_T_4, P_T_5, P_T_6, P_T_7, P_T_8, P_T_9)) := P in
+let '((Q_X_0, Q_X_1, Q_X_2, Q_X_3, Q_X_4, Q_X_5, Q_X_6, Q_X_7, Q_X_8, Q_X_9), (Q_Y_0, Q_Y_1, Q_Y_2, Q_Y_3, Q_Y_4, Q_Y_5, Q_Y_6, Q_Y_7, Q_Y_8, Q_Y_9), (Q_Z_0, Q_Z_1, Q_Z_2, Q_Z_3, Q_Z_4, Q_Z_5, Q_Z_6, Q_Z_7, Q_Z_8, Q_Z_9), (Q_T_0, Q_T_1, Q_T_2, Q_T_3, Q_T_4, Q_T_5, Q_T_6, Q_T_7, Q_T_8, Q_T_9)) := Q in
+_).
+    repeat match goal with
+             [x:?T |- _] =>
+             lazymatch T with
+             | Z => fail
+             | _ => clear x
+             end
+           end.
+
+    eexists.
+    cbv beta delta [ge25519_add'].
+    Reify_rhs.
+    reflexivity.
   Defined.
 
-  Definition and_ex_str :=
-    (Pipeline.toString (proj1_sig and_example)).
-
-  Definition mult_example: @pseudeq 32 W32 1 1 (fun v =>
-      plet a := $$ 1 in
-      plet b := v[[0]] in
-
-      (* NOTE: we want the lets in this format to unify with
-               pseudo_mult_dual *)
-      plet c := multHigh a b in
-      plet d := a ^* b in
-
-      [b ^& d]).
-    pseudo_solve.
-  Defined.
-
-  Definition mult_ex_str :=
-    (Pipeline.toString (proj1_sig mult_example)).
-
-  Definition comb_example: @pseudeq 32 W32 1 1 (fun v =>
-      plet a := $$ 7 in
-      plet b := v[[0]] in
-      ([b ^& a; a ^+ b])).
-    pseudo_solve.
-  Admitted.
-
-  Definition comb_ex_str :=
-    (Pipeline.toString (proj1_sig comb_example)).
-  *)
-
-End PipelineExamples.
+  Definition ge25519_result_range := RangeInterp (ZToRange 32 ge25519_ast). *)
+End GF25519.
