src/Assembly/Compile.v
@@ -1,0 +1,310 @@
+Require Import Coq.Logic.Eqdep.
+Require Import Compare_dec Sumbool.
+Require Import PeanoNat Omega.
+
+Require Import Crypto.Assembly.PhoasCommon.
+Require Import Crypto.Assembly.HL.
+Require Import Crypto.Assembly.LL.
+Require Import Crypto.Assembly.QhasmEvalCommon.
+Require Import Crypto.Assembly.QhasmCommon.
+Require Import Crypto.Assembly.Qhasm.
+
+Module CompileHL.
+  Context {ivar : type -> Type}.
+  Context {ovar : Type}.
+
+  Fixpoint compile {t} (e:@HL.expr Z (@LL.arg Z Z) t) : @LL.expr Z Z t :=
+    match e with
+    | HL.Const n => LL.Return (LL.Const n)
+    | HL.Var _ arg => LL.Return arg
+    | HL.Binop t1 t2 t3 op e1 e2 =>
+       LL.under_lets (@compile _ e1) (fun arg1 =>
+          LL.under_lets (@compile _ e2) (fun arg2 =>
+            LL.LetBinop op arg1 arg2 (fun v =>
+              LL.Return v)))
+    | HL.Let _ ex _ eC =>
+       LL.under_lets (@compile _ ex) (fun arg => @compile _ (eC arg))
+    | HL.Pair t1 e1 t2 e2 =>
+       LL.under_lets (@compile _ e1) (fun arg1 =>
+          LL.under_lets (@compile _ e2) (fun arg2 =>
+             LL.Return (LL.Pair arg1 arg2)))
+    | HL.MatchPair _ _ ep _ eC =>
+        LL.under_lets (@compile _ ep) (fun arg =>
+          let (a1, a2) := LL.match_arg_Prod arg in @compile _ (eC a1 a2))
+    end.
+
+  Section Correctness.
+    Lemma compile_correct {_: Evaluable Z} {t} e1 e2 G (wf:HL.wf G e1 e2) :
+      List.Forall (fun v => let 'existT _ (x, a) := v in LL.interp_arg a = x) G ->
+        LL.interp (compile e2) = HL.interp e1 :> interp_type t.
+    Proof.
+      induction wf;
+        repeat match goal with
+        | [HIn:In ?x ?l, HForall:Forall _ ?l |- _ ] =>
+          (pose proof (proj1 (Forall_forall _ _) HForall _ HIn); clear HIn)
+        | [ H : LL.match_arg_Prod _ = (_, _) |- _ ] =>
+          apply LL.match_arg_Prod_correct in H
+        | [ H : LL.Pair _ _ = LL.Pair _ _ |- _ ] =>
+          apply LL.Pair_eq in H
+        | [ H : (_, _) = (_, _) |- _ ] => inversion H; clear H
+        | _ => progress intros
+        | _ => progress simpl in *
+        | _ => progress subst
+        | _ => progress specialize_by assumption
+        | _ => progress break_match
+        | _ => rewrite !LL.interp_under_lets
+        | _ => rewrite !LL.interp_arg_uninterp_arg
+        | _ => progress erewrite_hyp !*
+        | _ => apply Forall_cons
+        | _ => solve [intuition (congruence || eauto)]
+        end.
+    Qed.
+  End Correctness.
+End CompileHL.
+
+Module CompileLL.
+  Import LL Qhasm.
+  Import QhasmUtil ListNotations.
+
+  Section Compile.
+    Context {n: nat} {w: Width n}.
+
+    Definition WArg t': Type := @LL.arg (word n) (word n) t'.
+    Definition WExpr t': Type := @LL.expr (word n) (word n) t'.
+
+    Fixpoint LLProgram t (inputs: nat): Type :=
+      match inputs with
+      | (S m) => WArg TT -> @LLProgram t m
+      | O => WExpr t
+      end.
+
+    Section Mappings.
+      Definition indexize (x: nat) : Index n.
+        intros; destruct (le_dec n 0).
+
+        - exists 0; abstract intuition auto with zarith.
+        - exists (x mod n)%nat.
+            abstract (pose proof (Nat.mod_bound_pos x n);
+                    omega).
+      Defined.
+
+      Definition getMapping (x: WArg TT) :=
+        match x with
+        | Const v => constM n (@constant n w v)
+        | Var v => regM n (@reg n w (wordToNat v))
+        end.
+
+      Definition getReg (x: Mapping n): option (Reg n) :=
+        match x with | regM r => Some r | _ => None end.
+
+      Definition getConst (x: Mapping n): option (QhasmCommon.Const n) :=
+        match x with | constM c => Some c | _ => None end.
+
+      Definition makeA (output input: Mapping n): option Assignment :=
+        match (output, input) with
+        | (regM r, constM c) => Some (AConstInt r c)
+        | (regM r0, regM r1) => Some (ARegReg r0 r1)
+        | _ => None
+        end.
+
+      Definition makeOp {t1 t2 t3} (op: binop t1 t2 t3) (out in1 in2: Mapping n):
+            option (Reg n * option Assignment * Operation) :=
+        let mov :=
+          if (EvalUtil.mapping_dec out in1)
+          then None
+          else makeA out in1 in
+
+        match op with
+        | OPadd =>
+          omap (getReg out) (fun r0 =>
+            match in2 with
+            | regM r1 => Some (r0, mov, IOpReg IAdd r0 r1)
+            | constM c => Some (r0, mov, IOpConst IAdd r0 c)
+            | _ => None
+            end)
+
+        | OPsub =>
+          omap (getReg out) (fun r0 =>
+            match in2 with
+            | regM r1 => Some (r0, mov, IOpReg ISub r0 r1)
+            | constM c => Some (r0, mov, IOpConst ISub r0 c)
+            | _ => None
+            end)
+
+        | OPmul => 
+          omap (getReg out) (fun r0 =>
+            match in2 with
+            | regM r1 => Some (r0, mov, DOp Mult r0 r1 None)
+            | _ => None
+            end)
+
+        | OPand =>
+          omap (getReg out) (fun r0 =>
+            match in2 with
+            | regM r1 => Some (r0, mov, IOpReg IAnd r0 r1)
+            | constM c => Some (r0, mov, IOpConst IAnd r0 c)
+            | _ => None
+            end)
+
+        | OPshiftr => 
+          omap (getReg out) (fun r0 =>
+            match in2 with
+            | constM (constant _ _ w) =>
+                Some (r0, mov, ROp Shr r0 (indexize (wordToNat w)))
+            | _ => None
+            end)
+        end.
+    End Mappings.
+
+    Section TypeDec.
+      Fixpoint type_eqb (t0 t1: type): bool :=
+        match (t0, t1) with
+        | (TT, TT) => true
+        | (Prod t0a t0b, Prod t1a t1b) => andb (type_eqb t0a t1a) (type_eqb t0b t1b)
+        | _ => false
+        end.
+
+      Lemma type_eqb_spec: forall t0 t1, type_eqb t0 t1 = true <-> t0 = t1.
+      Proof.
+        intros; split.
+
+        - revert t1; induction t0 as [|t0a IHt0a t0b IHt0b].
+
+            + induction t1; intro H; simpl in H; inversion H; reflexivity.
+
+            + induction t1; intro H; simpl in H; inversion H.
+            apply andb_true_iff in H; destruct H as [Ha Hb].
+
+            apply IHt0a in Ha; apply IHt0b in Hb; subst.
+            reflexivity.
+
+        - intro H; subst.
+            induction t1; simpl; [reflexivity|]; apply andb_true_iff; intuition.
+      Qed.
+
+      Definition type_dec (t0 t1: type): {t0 = t1} + {t0 <> t1}.
+        refine (match (type_eqb t0 t1) as b return _ = b -> _ with
+            | true => fun e => left _
+            | false => fun e => right _
+            end eq_refl);
+        [ abstract (apply type_eqb_spec in e; assumption)
+        | abstract (intro H; apply type_eqb_spec in H;
+                    rewrite e in H; contradict H; intro C; inversion C) ].
+      Defined.
+    End TypeDec.
+
+    Fixpoint vars {t} (a: WArg t): list nat :=
+      match t as t' return WArg t' -> list nat with
+      | TT => fun a' =>
+        match a' with
+        | Var v' => [wordToNat v']
+        | _ => @nil nat
+        end
+      | Prod t0 t1 => fun a' =>
+        match a' with
+        | Pair _ _ a0 a1 => (vars a0) ++ (vars a1)
+        end
+      end a.
+
+    Definition getOutputSlot {t} (nextRegName: nat) (op: binop TT TT TT) (x y: WArg TT)
+               (eC: WArg TT -> WExpr t) : option nat :=
+      match (makeOp op (regM _ (reg w nextRegName)) (getMapping x) (getMapping y)) with
+      | Some (reg _ _ r, Some a, op') => Some r
+      | Some (reg _ _ r, None, op')   => Some r
+      | _                             => None
+      end.
+
+    Section ExprF.
+      Context (Out: Type)
+              (update: binop TT TT TT -> WArg TT -> WArg TT -> Out -> option Out)
+              (get: forall t', WArg t' -> option Out).
+
+      Fixpoint zeros (t: type): WArg t :=
+        match t with
+        | TT => Const (@wzero n)
+        | Prod t0 t1 => Pair (zeros t0) (zeros t1)
+        end.
+ 
+      Fixpoint depth {t} (p: WExpr t) {struct p}: nat :=
+        match p with
+        | LetBinop _ _ _ _ _ _ t' eC => S (depth (eC (zeros _)))
+        | Return _ a => O
+        end.
+
+      Fixpoint exprF0 t d (nextVar: nat) (p: {e: WExpr t | depth e = d}) {struct d}: option Out.
+        refine (match d as d' return {e: WExpr t | depth e = d'} -> _ with
+        | (S m) => fun p' =>
+          match proj1_sig p' with
+          | LetBinop TT TT TT op x y t' eC =>
+            omap (getOutputSlot nextVar op x y eC) (fun r =>
+              omap (exprF0 t' m (S nextVar) (exist _ (eC (Var (@natToWord n r))) _)) (fun o =>
+                update op x y o))
+          | _ => None
+          end
+        | O => fun p' =>
+          match proj1_sig p' with
+          | Return _ a => get _ a
+          | _ => None
+          end
+        end p).
+
+        destruct p' as [p' D'], p'; simpl in D'.
+        inversion D'; subst.
+      Admitted.
+
+      Fixpoint exprF1 t inputs (args: list nat) (p: LLProgram t inputs): option Out.
+        refine (match inputs as i' return LLProgram t i' -> _ with
+        | (S m) => fun p' => @exprF Out t m update get (cons inputs args)
+                                (p' (@Var (word n) (word n) (@natToWord n nextVar)))
+        | O => fun p' =>
+        end p).
+        Defined.
+    Section ExprF.
+
+    Fixpoint exprF {t Out}
+        
+        t) (e: @LL.expr (word n) nat t) {struct e}: option Out :=
+      match e with
+      | LetBinop TT TT TT op x y t' eC =>
+        omap (getOutputSlot nextRegName op x y eC) (fun r =>
+          omap (exprF update get (S nextRegName) (eC (Var r))) (fun out =>
+            update op x y out))
+      | Return _ a => get _ a
+      | _ => None
+      end.
+
+    Fixpoint getProg {t} :=
+      @exprF t Program
+        (fun op x y out ->
+            match (makeOp op (regM _ (reg w nextRegName)) (@getMapping n w x) (@getMapping n w y)) with
+            | Some (reg _ _ r, Some a, op') => Some ((QAssign a) :: (QOp op') :: out)
+            | Some (reg _ _ r, None, op')   => Some ((QOp op') :: out)
+            | _                             => None
+            end)
+        (fun t' a => [])
+
+    Fixpoint getOuts {t} :=
+      @exprF t Program
+        (fun op x y out -> Some out)
+        (fun t' a => vars a)
+
+      match e with
+      | LetBinop TT TT TT op x y t' eC =>
+        if (type_dec t t')
+        then match compile'' nextRegName op x y _ with
+          | Some (progHead, outputVar, nextRegName') =>
+            match compile' nextRegName' (_ op eC) with
+            | Some (progTail, outputs) => Some (progHead ++ progTail, outputs)
+            | None => None
+            end
+          | None => None
+          end
+        else None
+      | Return _ a => Some ([], vars a)
+      | _ => None
+      end.
+
+    Definition compile {t inputs} (prog: @LLProgram _ t inputs): option (Program * list nat) :=
+      @compile' t inputs (freeVars prog).
+  End Compile.
+End CompileLL.
