src/Assembly/Conversions.v
@@ -1,0 +1,373 @@
+Require Import Crypto.Assembly.PhoasCommon.
+
+Require Export Crypto.Assembly.QhasmUtil.
+Require Export Crypto.Assembly.QhasmEvalCommon.
+Require Export Crypto.Assembly.WordizeUtil.
+Require Export Crypto.Assembly.Evaluables.
+Require Export Crypto.Assembly.HL.
+Require Export Crypto.Assembly.LL.
+
+Require Export FunctionalExtensionality.
+
+Require Import Bedrock.Nomega.
+
+Require Import Coq.ZArith.ZArith_dec.
+Require Import Coq.ZArith.Znat.
+
+Module HLConversions.
+  Import HL.
+
+  Definition convertVar {A B: Type} {EA: Evaluable A} {EB: Evaluable B} {t} (a: interp_type (T := A) t): interp_type (T := B) t.
+  Proof.
+    induction t as [| t3 IHt1 t4 IHt2].
+
+    - refine (@toT B EB (@fromT A EA _)); assumption.
+
+    - destruct a as [a1 a2]; constructor;
+        [exact (IHt1 a1) | exact (IHt2 a2)].
+  Defined.
+
+  Fixpoint convertExpr {A B: Type} {EA: Evaluable A} {EB: Evaluable B} {t v} (a: expr (T := A) (var := v) t): expr (T := B) (var := v) t :=
+    match a with
+    | Const x => Const (@toT B EB (@fromT A EA x))
+    | Var t x => @Var B _ t x
+    | Binop t1 t2 t3 o e1 e2 =>
+      @Binop B _ t1 t2 t3 o (convertExpr e1) (convertExpr e2)
+    | Let tx e tC f =>
+      Let (convertExpr e) (fun x => convertExpr (f x))
+    | Pair t1 e1 t2 e2 => Pair (convertExpr e1) (convertExpr e2)
+    | MatchPair t1 t2 e tC f => MatchPair (convertExpr e) (fun x y =>
+        convertExpr (f x y))
+    end.
+
+  Fixpoint convertExpr' {A B: Type} {EA: Evaluable A} {EB: Evaluable B} {t} (a: expr (T := A) (var := @interp_type A) t): expr (T := B) (var := @interp_type B) t :=
+    match a with
+    | Const x => Const (@toT B EB (@fromT A EA x))
+    | Var t x => @Var B _ t (convertVar x)
+    | Binop t1 t2 t3 o e1 e2 =>
+      @Binop B _ t1 t2 t3 o (convertExpr' e1) (convertExpr' e2)
+    | Let tx e tC f =>
+      Let (convertExpr' e) (fun x => convertExpr' (f (convertVar x)))
+    | Pair t1 e1 t2 e2 => Pair (convertExpr' e1) (convertExpr' e2)
+    | MatchPair t1 t2 e tC f => MatchPair (convertExpr' e) (fun x y =>
+        convertExpr' (f (convertVar x) (convertVar y)))
+    end.
+
+  Definition convertZToWord {t} n v a :=
+    @convertExpr Z (word n) ZEvaluable (@WordEvaluable n) t v a.
+
+  Definition convertZToWordRangeOpt {t} n v a :=
+    @convertExpr Z (@WordRangeOpt n) ZEvaluable (@WordRangeOptEvaluable n) t v a.
+
+  Definition convertZToWord' {t} n a :=
+    @convertExpr' Z (word n) ZEvaluable (@WordEvaluable n) t a.
+
+  Definition convertZToWordRangeOpt' {t} n a :=
+    @convertExpr' Z (@WordRangeOpt n) ZEvaluable (@WordRangeOptEvaluable n) t a.
+
+  Definition ZToWord {t} n (a: @Expr Z t): @Expr (word n) t :=
+    fun v => convertZToWord n v (a v).
+
+  Definition ZToRange {t} n (a: @Expr Z t): @Expr (@WordRangeOpt n) t :=
+    fun v => convertZToWordRangeOpt n v (a v).
+
+  Definition typeMap {A B t} (f: A -> B) (x: @interp_type A t): @interp_type B t.
+  Proof.
+    induction t; [refine (f x)|].
+    destruct x as [x1 x2].
+    refine (IHt1 x1, IHt2 x2).
+  Defined.
+
+  Definition RangeInterp {n t} E: @interp_type (option (Range N)) t :=
+    typeMap rangeEval (@Interp (@WordRangeOpt n) (@WordRangeOptEvaluable n) t E).
+
+  Example example_Expr : Expr TT := fun var => (
+    Let (Const 7) (fun a =>
+      Let (Let (Binop OPadd (Var a) (Var a)) (fun b => Pair (Var b) (Var b))) (fun p =>
+        MatchPair (Var p) (fun x y =>
+          Binop OPadd (Var x) (Var y)))))%Z.
+
+  Example interp_example_range :
+    RangeInterp (ZToRange 32 example_Expr) = Some (range N 28%N 28%N).
+  Proof. reflexivity. Qed.
+End HLConversions.
+
+Module LLConversions.
+  Import LL.
+
+  Definition convertVar {A B: Type} {EA: Evaluable A} {EB: Evaluable B} {t} (a: interp_type (T := A) t): interp_type (T := B) t.
+  Proof.
+    induction t as [| t3 IHt1 t4 IHt2].
+
+    - refine (@toT B EB (@fromT A EA _)); assumption.
+
+    - destruct a as [a1 a2]; constructor;
+        [exact (IHt1 a1) | exact (IHt2 a2)].
+  Defined.
+
+  Fixpoint convertArg {A B: Type} {EA: Evaluable A} {EB: Evaluable B} {t} (x: arg (T := A) t): arg (T := B) t :=
+    match x with | Arg t' c => Arg t' (convertVar (t := t') c) end.
+
+  Fixpoint convertExpr {A B: Type} {EA: Evaluable A} {EB: Evaluable B} {t} (a: expr (T := A) t): expr (T := B) t :=
+    match a with
+    | LetBinop _ _ out op a b _ eC =>
+      LetBinop (T := B) op (convertArg a) (convertArg b) (fun x: (interp_type (T := B) out) => convertExpr (eC (convertVar x)))
+    | Return _ a => Return (convertArg a)
+    end.
+
+  Definition convertZToWord {t} n a :=
+    @convertExpr Z (word n) ZEvaluable (@WordEvaluable n) t a.
+
+  Definition convertZToWordRangeOpt {t} n a :=
+    @convertExpr Z (@WordRangeOpt n) ZEvaluable (@WordRangeOptEvaluable n) t a.
+
+  Definition typeMap {A B t} (f: A -> B) (x: @interp_type A t): @interp_type B t.
+  Proof.
+    induction t; [refine (f x)|].
+    destruct x as [x1 x2].
+    refine (IHt1 x1, IHt2 x2).
+  Defined.
+
+  Definition zinterp {t} E := @interp Z ZEvaluable t E.
+
+  Definition wordInterp {n t} E := @interp (word n) (@WordEvaluable n) t E.
+
+  Definition rangeInterp {n t} E: @interp_type (@WordRangeOpt n) t :=
+    @interp (@WordRangeOpt n) (@WordRangeOptEvaluable n) t E.
+
+  Section Correctness.
+    (* Aliases to make the proofs easier to read. *)
+
+    Definition varZToRange {n t} (v: @interp_type Z t): @interp_type (@WordRangeOpt n) t :=
+      @convertVar Z (@WordRangeOpt n) ZEvaluable (WordRangeOptEvaluable) t v.
+
+    Definition varRangeToZ {n t} (v: @interp_type (@WordRangeOpt n) t): @interp_type Z t :=
+      @convertVar (@WordRangeOpt n) Z (WordRangeOptEvaluable) ZEvaluable t v.
+
+    Definition varZToWord {n t} (v: @interp_type Z t): @interp_type (@word n) t :=
+      @convertVar Z (@word n) ZEvaluable (@WordEvaluable n) t v.
+
+    Definition varWordToZ {n t} (v: @interp_type (@word n) t): @interp_type Z t :=
+      @convertVar (word n) Z (@WordEvaluable n) ZEvaluable t v.
+
+    Definition zOp {tx ty tz: type} (op: binop tx ty tz)
+               (x: @interp_type Z tx) (y: @interp_type Z ty): @interp_type Z tz :=
+      @interp_binop Z ZEvaluable _ _ _ op x y.
+
+    Definition wordOp {n} {tx ty tz: type} (op: binop tx ty tz)
+               (x: @interp_type _ tx) (y: @interp_type _ ty): @interp_type _ tz :=
+      @interp_binop (word n) (@WordEvaluable n) _ _ _ op x y.
+
+    Definition rangeOp {n} {tx ty tz: type} (op: binop tx ty tz)
+               (x: @interp_type _ tx) (y: @interp_type _ ty): @interp_type _ tz :=
+      @interp_binop (@WordRangeOpt n) (@WordRangeOptEvaluable n) _ _ _ op x y.
+
+    Definition rangeArg {n t} (x: @arg (@WordRangeOpt n) t) := @interp_arg _ _ x.
+
+    Definition wordArg {n t} (x: @arg (word n) t) := @interp_arg _ _ x.
+
+
+    (* Bounds-checking fixpoint *)
+
+    Fixpoint checkVar {n t} (x: @interp_type (@WordRangeOpt n) t) :=
+      match t as t' return (interp_type t') -> Prop with
+      | TT => fun x' =>
+        match (rangeEval x') with
+        | Some (range low high) => True
+        | None => False
+        end
+      | Prod t0 t1 => fun x' =>
+        match x' with
+        | (x0, x1) => (checkVar (n := n) x0) /\ (checkVar (n := n) x1)
+        end
+      end x.
+
+    Fixpoint check {n t} (e : @expr (@WordRangeOpt n) t): Prop :=
+      match e with
+      | LetBinop ta tb tc op a b _ eC =>
+          (@checkVar n tc (rangeOp op (interp_arg a) (interp_arg b)))
+        /\ (check (eC (rangeOp op (interp_arg a) (interp_arg b))))
+      | Return _ a => checkVar (interp_arg a)
+      end.
+
+    (* Utility Lemmas *)
+
+    Lemma interp_arg_convert : forall {A B t} {EA: Evaluable A} {EB: Evaluable B} (x: @arg A t),
+        (interp_arg (@convertArg A B EA EB t x)) = @convertVar A B EA EB t (interp_arg x).
+    Proof. induction x as [t i]; induction t, EA, EB; simpl; reflexivity. Qed.
+
+    Lemma ZToRange_binop_correct : forall {n tx ty tz} (op: binop tx ty tz) (x: @arg _ tx) (y: @arg _ ty) e,
+        check (t := tz) (convertZToWordRangeOpt n (LetBinop op x y e))
+      -> zOp op (interp_arg x) (interp_arg y) =
+          varRangeToZ (rangeOp (n := n) op (varZToRange (interp_arg x)) (varZToRange (interp_arg y))).
+    Proof.
+      intros until e; intro H.
+      unfold convertZToWordRangeOpt, convertExpr, check, rangeOp in H.
+      repeat rewrite interp_arg_convert in H; simpl in H.
+      destruct H as [H H0]; clear H0.
+
+      induction op; unfold zOp, varRangeToZ, rangeOp.
+
+      - simpl; unfold getUpperBoundOpt.
+        repeat rewrite interp_arg_convert in H; simpl in H.
+        unfold id, makeRange in *.
+        repeat match goal with
+        | [|- context[Z_le_dec ?a ?b] ] => destruct (Z_le_dec a b)
+        | [|- context[Z_lt_dec ?a ?b] ] => destruct (Z_lt_dec a b)
+        end; simpl in H; intuition.
+
+        rewrite applyBinOp_constr_spec; simpl.
+        rewrite applyBinOp_constr_spec in H; simpl in H.
+        destruct (overflows n _); [intuition|]; simpl.
+
+    Admitted.
+
+    Lemma ZToWord_binop_correct : forall {n tx ty tz} (op: binop tx ty tz) (x: @arg _ tx) (y: @arg _ ty) e,
+        check (t := tz) (convertZToWordRangeOpt n (LetBinop op x y e))
+      -> zOp op (interp_arg x) (interp_arg y) =
+          varWordToZ (wordOp (n := n) op (varZToWord (interp_arg x)) (varZToWord (interp_arg y))).
+    Proof.
+      intros until e; intro H.
+      unfold convertZToWordRangeOpt, convertExpr, check, rangeOp in H.
+      repeat rewrite interp_arg_convert in H; simpl in H.
+      destruct H as [H H0]; clear H0.
+
+      induction op; unfold zOp, varRangeToZ, rangeOp.
+
+      - simpl; unfold getUpperBoundOpt; simpl in H.
+        rewrite applyBinOp_constr_spec in H; simpl in H.
+
+        unfold makeRange in H.
+        repeat match goal with
+        | [ H : context[Z_le_dec ?a ?b] |- _ ] => destruct (Z_le_dec a b)
+        | [ H : context[Z_lt_dec ?a ?b] |- _ ] => destruct (Z_lt_dec a b)
+        end; simpl in H; intuition.
+
+        unfold id in *.
+        destruct (QhasmUtil.overflows n (Z.to_N (interp_arg x) + Z.to_N (interp_arg y)));
+            [intuition|]; simpl.
+
+        rewrite <- wordize_plus.
+
+        + repeat rewrite wordToN_NToWord; try assumption;
+            try abstract (apply N2Z.inj_lt; rewrite Z2N.id; assumption).
+
+          rewrite N2Z.inj_add.
+          repeat rewrite Z2N.id; try assumption.
+          reflexivity.
+
+        + repeat rewrite wordToN_NToWord; [assumption | |];
+              rewrite N2Z.inj_lt;
+              repeat rewrite Z2N.id;
+              try assumption.
+    Admitted.
+
+    (* Main correctness guarantee *)
+
+    Lemma RangeInterp_correct: forall {n t} (E: @expr Z t),
+        check (convertZToWordRangeOpt n E)
+      -> typeMap (fun x => NToWord n (Z.to_N x)) (zinterp E) = wordInterp (convertZToWord n E).
+    Proof.
+      intros n t E S.
+      unfold rangeInterp, convertZToWordRangeOpt, zinterp,
+             convertZToWord, wordInterp.
+
+      induction E as [tx ty tz op x y z|]; simpl; try reflexivity.
+
+      - rewrite H.
+
+        + repeat f_equal; unfold id in *.
+          destruct x as [tx' x], y as [ty' y]; simpl.
+
+          destruct S as [S0 S1].
+
+          pose proof (ZToWord_binop_correct (n := n) op (Arg _ x) (Arg _ y)) as C;
+            unfold zOp, wordOp, varWordToZ, varZToWord in C; simpl in C.
+
+          induction op; rewrite (C (fun _ => Return (Arg TT 0%Z)));
+            repeat f_equal; split; try assumption; simpl; unfold makeRange;
+
+            repeat match goal with
+            | [|- context[Z_le_dec ?a ?b] ] => destruct (Z_le_dec a b)
+            | [|- context[Z_lt_dec ?a ?b] ] => destruct (Z_lt_dec a b)
+            end;
+
+            simpl; clear H S0 S1 C e; unfold id in *;
+            pose proof (Npow2_gt0 n) as H;
+            rewrite N2Z.inj_lt in H; simpl in H; intuition;
+
+            match goal with
+            | [A: (0 <= 0)%Z -> False |- _] =>
+              apply A; cbv; intro Q; inversion Q
+            end.
+
+        + destruct S as [S0 S1]; unfold convertZToWordRangeOpt.
+
+          replace (interp_binop op _ _)
+             with (varRangeToZ (rangeOp op
+                    (rangeArg (@convertArg _ _ ZEvaluable (@WordRangeOptEvaluable n) _ x))
+                    (rangeArg (@convertArg _ _ ZEvaluable (@WordRangeOptEvaluable n) _ y))));
+            [unfold varRangeToZ, rangeArg; assumption | clear S1].
+
+          destruct x as [tx' x], y as [ty' y]; simpl.
+
+          pose proof (ZToRange_binop_correct (n := n) op (Arg _ x) (Arg _ y)) as C;
+            unfold zOp, wordOp, varZToRange, varRangeToZ, convertZToWordRangeOpt in *;
+            simpl in C.
+
+          induction op; rewrite C with (e := fun _ => Return (Arg TT 0%Z));
+            split; try assumption; simpl; unfold makeRange;
+            repeat match goal with
+            | [|- context[Z_le_dec ?a ?b] ] => destruct (Z_le_dec a b)
+            | [|- context[Z_lt_dec ?a ?b] ] => destruct (Z_lt_dec a b)
+            end;
+
+            simpl; clear H S0 C e; unfold id in *;
+            pose proof (Npow2_gt0 n) as H;
+            rewrite N2Z.inj_lt in H; simpl in H; intuition;
+
+            match goal with
+            | [A: (0 <= 0)%Z -> False |- _] =>
+              apply A; cbv; intro Q; inversion Q
+            end.
+
+
+      - simpl in S.
+        induction a; simpl in *; try reflexivity.
+    Qed.
+  End Correctness.
+End LLConversions.
+
+Section ConversionTest.
+  Import HL HLConversions.
+
+  Fixpoint keepAddingOne {var} (x : @expr Z var TT) (n : nat) : @expr Z var TT :=
+    match n with
+    | O => x
+    | S n' => Let (Binop OPadd x (Const 1%Z)) (fun y => keepAddingOne (Var y) n')
+    end.
+
+  Definition KeepAddingOne (n : nat) : Expr (T := Z) TT :=
+    fun var => keepAddingOne (Const 1%Z) n.
+
+  Definition testCase := Eval vm_compute in KeepAddingOne 4000.
+
+  Eval vm_compute in RangeInterp (ZToRange 0 testCase).
+  Eval vm_compute in RangeInterp (ZToRange 1 testCase).
+  Eval vm_compute in RangeInterp (ZToRange 10 testCase).
+  Eval vm_compute in RangeInterp (ZToRange 32 testCase).
+  Eval vm_compute in RangeInterp (ZToRange 64 testCase).
+  Eval vm_compute in RangeInterp (ZToRange 128 testCase).
+
+  Definition nefarious : Expr (T := Z) TT :=
+    fun var => Let (Binop OPadd (Const 10%Z) (Const 20%Z))
+                   (fun y => Binop OPmul (Var y) (Const 0%Z)).
+
+  Eval vm_compute in RangeInterp (ZToRange 0 nefarious).
+  Eval vm_compute in RangeInterp (ZToRange 1 nefarious).
+  Eval vm_compute in RangeInterp (ZToRange 4 nefarious).
+  Eval vm_compute in RangeInterp (ZToRange 5 nefarious).
+  Eval vm_compute in RangeInterp (ZToRange 32 nefarious).
+  Eval vm_compute in RangeInterp (ZToRange 64 nefarious).
+  Eval vm_compute in RangeInterp (ZToRange 128 nefarious).
+End ConversionTest.
